StrataTest/Languages/Boole/find_max_verus.lean
@@ -98,27 +98,27 @@ Obligation: witnessOccurs_ensures_2_1229
 Property: assert
 Result: ✅ pass
 
-Obligation: entry_invariant_0_0
+Obligation: loopElimAssert_loop_7_entry_invariant_0
 Property: assert
 Result: ✅ pass
 
-Obligation: entry_invariant_0_1
+Obligation: loopElimAssert_loop_7_entry_invariant_1
 Property: assert
 Result: ✅ pass
 
-Obligation: entry_invariant_0_2
+Obligation: loopElimAssert_loop_7_entry_invariant_2
 Property: assert
 Result: ✅ pass
 
-Obligation: arbitrary_iter_maintain_invariant_0_0
+Obligation: loopElimAssert_loop_7_arbitrary_iter_maintain_invariant_0
 Property: assert
 Result: ✅ pass
 
-Obligation: arbitrary_iter_maintain_invariant_0_1
+Obligation: loopElimAssert_loop_7_arbitrary_iter_maintain_invariant_1
 Property: assert
 Result: ✅ pass
 
-Obligation: arbitrary_iter_maintain_invariant_0_2
+Obligation: loopElimAssert_loop_7_arbitrary_iter_maintain_invariant_2
 Property: assert
 Result: ✅ pass
 
